Reducing multi-tape halting on one tape to single-tape halting

theories/PCP/singleTM.v
@@ -1,164 +1,13 @@
 Require Export Undecidability.Shared.Prelim.
+Require Export PslBase.FiniteTypes.
+Require Export TM.LM.HaltingProblem.
+Require Export TM.TM.
+Require Import Equations.Equations.
+Require Import Problems.Reduction.
+
+Derive Signature for vector.
 
 (** * TM to SRH *)
-
-(* ** More preliminaries, with definition of finite types *)
-
-Definition dec (X: Prop) : Type := {X} + {~ X}.
-Coercion dec2bool P (d: dec P) := if d then true else false.
-Existing Class dec.
-Definition Dec (X: Prop) (d: dec X) : dec X := d.
-Arguments Dec X {d}.
-
-Hint Extern 4 =>  (* Improves type class inference *)
-match goal with
-  | [  |- dec ((fun _ => _) _) ] => cbn
-end : typeclass_instances.
-
-Tactic Notation "decide" constr(p) :=
-  destruct (Dec p).
-Tactic Notation "decide" constr(p) "as" simple_intropattern(i) :=
-  destruct (Dec p) as i.
-Tactic Notation "decide" "_" :=
-  destruct (Dec _).
-
-Notation "'eq_dec' X" := (forall x y : X, dec (x=y)) (at level 70).
-
-Structure eqType := EqType {
-  eqType_X :> Type;
-  eqType_dec : eq_dec eqType_X }.
-
-Arguments EqType X {_} : rename.
-Canonical Structure eqType_CS X (A: eq_dec X) := EqType X.
-Existing Instance eqType_dec.
-
-Instance list_eq_dec X :
-  eq_dec X -> eq_dec (list X).
-Proof.
-  unfold dec. decide equality.
-Defined.
-
-(** The definitions of finite types are adopted from the Bachelor Thesis of Jan Menz. (https://www.ps.uni-saarland.de/~menz/bachelor.php) *)
-
-Fixpoint count (X: Type) `{eq_dec X}  (A: list  X) (x:  X) {struct A} : nat :=
-  match A with
-  | nil => O
-  | cons y A' =>  if Dec (x=y) then S(count A' x) else count A' x end.
-
-Class finTypeC  (type:eqType) : Type := FinTypeC {
-                                            enum: list type;
-                                            enum_ok: forall x: type, count enum x = 1
-                                          }.
-
-Structure finType : Type := FinType {
-                                type:> eqType;
-                                class: finTypeC type }.
-
-Arguments FinType type {class}.
-Existing Instance class | 0.
-
-Canonical Structure finType_CS (X : Type) {p : eq_dec X} {class : finTypeC (EqType X)} : finType := FinType (EqType X).
-
-Definition elem (F: finType) := @enum (type F) (class F).
-Hint Unfold elem.
-Hint Unfold class.
-
-Ltac dec := repeat (destruct Dec).
-
-Lemma countIn (X:eqType) (x:X) A:
-  count A x > 0 -> x el A.
-Proof.
-  induction A.
-  - cbn. omega.
-  - cbn. dec.
-    + intros. left. symmetry. exact e.
-    + intros. right. apply IHA. exact H.
-Qed.
-
-Lemma elem_spec (X: finType) (x:X) : x el (elem X).
-Proof.
-  apply countIn.  pose proof (enum_ok x) as H. unfold elem. omega.
-Qed.
-
-Hint Resolve elem_spec.
-Hint Resolve enum_ok.
-
-Lemma countSplit (X: eqType) (A B: list X) (x: X)  : count A x + count B x = count (A ++ B) x.
-Proof.
-  induction A.
-  - reflexivity.
-  - cbn. decide (x=a).
-    +cbn. f_equal; exact IHA.
-    + exact IHA.
-Qed.
-
-Fixpoint pos (X : eqType) (x : X) (A : list X) :=
-  match A with
-  | [] => None
-  | a :: A => if Dec (x = a) then Some 0 else match pos x A with Some n => Some (S n) | None => None end
-  end.
-
-Definition pos_el' (X : eqType) (x : X) (A : list X) (H : x el A) : {n | pos x A = Some n}.
-Proof.
-  induction A.
-  - inv H.
-  - decide (x = a).
-    + subst. exists 0. cbn. decide (a = a); congruence.
-    + destruct IHA; try firstorder congruence.
-      exists (S x0). cbn. decide (x = a); rewrite ?e; congruence.
-Defined.
-
-Lemma pos_length (X : eqType) (x : X) A n :
-  pos x A = Some n -> n < |A|.
-Proof.
-  revert n; induction A; cbn; intros.
-  - inv H.
-  - decide (x = a).
-    + inv H. omega.
-    + destruct (pos x A) eqn:E; inv H. specialize (IHA n1 eq_refl). omega.
-Qed.
-
-Lemma pos_nth (X : eqType) (x : X) A n :
-  pos x A = Some n -> nth_error A n = Some x.
-Proof.
-  revert n; induction A; cbn; intros.
-  - inv H.
-  - decide (x = a).
-    + now inv H.
-    + destruct (pos x A) eqn:E; inv H. cbn. eauto. 
-Qed.    
-
-Definition pos_el (X : eqType) (x : X) (A : list X) (H : x el A) := proj1_sig (pos_el' H).
-
-Definition index (X : finType) (x : X) := pos_el (elem_spec x).
-
-
-Lemma map_app_inv X Y (f : X -> Y) x y z :
-  map f x = y ++ z -> exists x' x'', x = x' ++ x'' /\ map f x' = y /\ map f x'' = z.
-Proof.
-  revert x; induction y; cbn; intros.
-  - exists [], x. firstorder.
-  - destruct x; inv H.
-    destruct (IHy _ H2) as (x' & x'' & -> & <- & <-).
-    exists (x :: x'), (x''). firstorder.
-Qed.
-
-Lemma pos_inj (X : eqType) (x y : X) (A : list X) n :
-  pos x A = Some n -> pos y A = Some n -> x = y.
-Proof.
-  revert n; induction A; cbn; intros.
-  - inv H.
-  - decide (x = a); decide (y = a); subst; try congruence.
-    + inv H. destruct (pos y A); inv H0.
-    + inv H0. destruct (pos x A); inv H.
-    + destruct (pos x A), (pos y A); inv H; inv H0. eauto.
-Qed.
-
-Lemma inj_index (X : finType) : Injective (@index X).
-Proof.
-  intros ? ? ?. unfold index, pos_el in *.
-  do 2 destruct pos_el'. cbn in H. subst. eapply pos_inj; eauto.
-Qed.
 
 (** ** Definition of single-tape Turing Machines  *)
 (** Adopted definitions from the formalization of Multitape Turing Machines taken from Asperti, Riciotti "Formalizing Turing Machines" and accompanying Matita foramlisation *)
@@ -177,20 +26,22 @@ symbol could be missing. This may happen for three different reasons: both tapes
 are empty; we are on the left extremity of a non-empty tape (left overflow), or 
 we are on the right extremity of a non-empty tape (right overflow). *)
   
-  Inductive tape : Type :=
-  | niltape : tape
-  | leftof : sig -> list sig -> tape
-  | rightof : sig -> list sig -> tape
-  | midtape : list sig -> sig -> list sig -> tape.
+  (* Inductive tape : Type := *)
+  (* | niltape : tape *)
+  (* | leftof : sig -> list sig -> tape *)
+  (* | rightof : sig -> list sig -> tape *)
+  (* | midtape : list sig -> sig -> list sig -> tape. *)
 
+  Notation tape := (tape sig).
+  
   Global Instance eq_dec_tape: eq_dec tape.
-  Proof. unfold dec. decide equality; decide (e=e0); decide (l=l0); auto;
-           decide (l= l1); decide (l0=l2); auto. 
+  Proof. unfold EqDec.dec. repeat decide equality.
+         all: eapply eqType_dec.
   Defined.
   
   Definition tapeToList (t : tape) : list sig :=
     match t with
-    | niltape => []
+    | niltape _ => []
     | leftof s r => s :: r
     | rightof s l => List.rev (s :: l)
     | midtape l c r => (List.rev l) ++ [c] ++ r 
@@ -198,33 +49,33 @@ we are on the right extremity of a non-empty tape (right overflow). *)
   
   Definition sizeOfTape t := |tapeToList t|.
 
-  (* symbol under head *)
-  Definition current :=
-    fun (t : tape) =>
-      match t with
-      | midtape _ c _ => Some c
-      | _ => None
-      end.
+  (* (* symbol under head *) *)
+  (* Definition current := *)
+  (*   fun (t : tape) => *)
+  (*     match t with *)
+  (*     | midtape _ c _ => Some c *)
+  (*     | _ => None *)
+  (*     end. *)
 
-  (* symbol-list left of head *)
-  Definition left :=
-    fun (t : tape) =>
-      match t with
-      | niltape => []
-      | leftof _ _ => []
-      | rightof s l => s :: l
-      | midtape l _ _ => l
-      end.
+  (* (* symbol-list left of head *) *)
+  (* Definition left := *)
+  (*   fun (t : tape) => *)
+  (*     match t with *)
+  (*     | niltape _ => [] *)
+  (*     | leftof _ _ => [] *)
+  (*     | rightof s l => s :: l *)
+  (*     | midtape l _ _ => l *)
+  (*     end. *)
 
-  (* symbol-list right of head *)
-  Definition right :=
-    fun (t : tape) =>
-      match t with
-      | niltape => []
-      | leftof s r => s :: r
-      | rightof _ _ => []
-      | midtape _ _ r => r
-      end.
+  (* (* symbol-list right of head *) *)
+  (* Definition right := *)
+  (*   fun (t : tape) => *)
+  (*     match t with *)
+  (*     | niltape _ => [] *)
+  (*     | leftof s r => s :: r *)
+  (*     | rightof _ _ => [] *)
+  (*     | midtape _ _ r => r *)
+  (*     end. *)
 
   (* makes a tape from left, current, right *)
    Definition mk_tape ls c rs :=
@@ -232,7 +83,7 @@ we are on the right extremity of a non-empty tape (right overflow). *)
     | Some c => midtape ls c rs
     | None => match ls with
              | List.nil => match rs with
-                     | List.nil => niltape
+                     | List.nil => niltape sig
                      | r :: rs => leftof r rs
                      end
              | l :: ls => rightof l ls
@@ -241,7 +92,7 @@ we are on the right extremity of a non-empty tape (right overflow). *)
 
   (* *** Definition of moves *)
   
-  Inductive move : Type := L : move | R : move | N : move.
+  (* Inductive move : Type := L : move | R : move | N : move. *)
 
   Global Instance move_eq_dec : eq_dec move.
   Proof.
@@ -266,32 +117,32 @@ we are on the right extremity of a non-empty tape (right overflow). *)
 
   (* Definition of tape movements *)
 
-  Definition tape_move_right :=
-    fun (t : tape) =>
-      match t with
-        niltape => niltape
-      | rightof _ _ =>t
-      | leftof a rs => midtape  [ ] a rs
-      | midtape ls a rs =>
-        match rs with
-          []  => rightof  a ls
-        | a0 :: rs0 => midtape (a::ls) a0 rs0
-        end
-      end.
+  (* Definition tape_move_right := *)
+  (*   fun (t : tape) => *)
+  (*     match t with *)
+  (*       niltape _ => niltape _ *)
+  (*     | rightof _ _ =>t *)
+  (*     | leftof a rs => midtape  [ ] a rs *)
+  (*     | midtape ls a rs => *)
+  (*       match rs with *)
+  (*         []  => rightof  a ls *)
+  (*       | a0 :: rs0 => midtape (a::ls) a0 rs0 *)
+  (*       end *)
+  (*     end. *)
 
 
-  Definition tape_move_left :=
-    fun (t : tape) =>
-      match t with 
-        niltape => niltape 
-      | leftof _ _ => t
-      | rightof a ls => midtape ls a [ ]
-      | midtape ls a rs => 
-        match ls with 
-          [] => leftof a rs
-        | a0 :: ls0 => midtape ls0 a0 (a::rs)
-        end
-      end.
+  (* Definition tape_move_left := *)
+  (*   fun (t : tape) => *)
+  (*     match t with  *)
+  (*       niltape _ => niltape _ *)
+  (*     | leftof _ _ => t *)
+  (*     | rightof a ls => midtape ls a [ ] *)
+  (*     | midtape ls a rs =>  *)
+  (*       match ls with  *)
+  (*         [] => leftof a rs *)
+  (*       | a0 :: ls0 => midtape ls0 a0 (a::rs) *)
+  (*       end *)
+  (*     end. *)
 
   Definition tape_move := fun (t : tape) (m : move) =>
                             match m with  R => tape_move_right t | L => tape_move_left t | N => t end.
@@ -299,7 +150,7 @@ we are on the right extremity of a non-empty tape (right overflow). *)
   (* Writing on the tape *)
 
   Definition tape_write := fun (t : tape) (s : option sig) =>
-                             match s with 
+                             match s with
                                None => t
                              | Some s0 => midtape (left t) s0 (right t)
                              end.
@@ -339,16 +190,16 @@ we are on the right extremity of a non-empty tape (right overflow). *)
     
   (* Run the machine i steps until it halts *)
   (* Returns None iff the maschine does not halt within i steps *)
-  Definition loop (A:Type) := fix l n (f:A -> A) (p : A -> bool) a {struct n}:=
-                              if p a then Some a  else
-                                match n with
-                                  O => None
-                                | S m => l m f p (f a)
-                                end.
+  (* Definition loop (A:Type) := fix l n (f:A -> A) (p : A -> bool) a {struct n}:= *)
+  (*                             if p a then Some a  else *)
+  (*                               match n with *)
+  (*                                 O => None *)
+  (*                               | S m => l m f p (f a) *)
+  (*                               end. *)
 
   
   Definition loopM := fun (M :sTM) (i : nat) cin =>
-                        loop i (@step M) (fun c => halt (cstate c)) cin. 
+                        loop (@step M) (fun c => halt (cstate c)) cin i. 
 
 
   
@@ -358,7 +209,7 @@ we are on the right extremity of a non-empty tape (right overflow). *)
     exists i outc, loopM i start = Some outc.
 
   Lemma loop_step_not A f p (a : A) i out:
-    loop i f p (f a) = out -> (p a = false) -> (loop (S i) f p a = out). 
+    loop f p (f a) i = out -> (p a = false) -> (loop f p a (S i) = out). 
   Proof.
   destruct i; intros H HF; cbn in *; rewrite HF; destruct (p (f a)); assumption.   
   Qed.
@@ -398,3 +249,55 @@ Definition Reach (S: (sigT (fun (sig:finType) =>
   let (c1,c2) := (projT2 (projT2 S)) in
   reach c1 c2. 
      
+
+Definition single_TM_halt : { sig : _ & (mTM sig 1) * (tapes sig 1)}%type -> Prop :=
+  fun '(existT _ sig (M, t)) => exists outc k, TM.loopM (TM.initc M t) k = Some outc.
+
+Equations (noeqns) f_config A B : TM.mconfig A B 1 -> mconfig A B :=
+  { f_config (TM.mk_mconfig a [|b|]) := mk_mconfig a b }.
+
+Require Import TM.Prelim.
+
+Lemma TM_conv : single_TM_halt ⪯ Halt.
+Proof.
+  unshelve eexists.
+  - intros [sig [[] t]]. do 2 depelim t.
+    exists sig. econstructor.
+    + intros []. destruct (trans0 (e, [| o |])) eqn:E.
+      do 2 depelim t.
+      exact (e0, h0).
+    + exact start0.
+    + exact halt0.
+    + exact h.
+  - intros [sig [[] t]]. cbn. do 2 depelim t; cbn.
+    unfold Halt. rewrite <- TM_terminates_Halt. cbn.
+    split.
+    + intros (? & ? & ?). 
+      destruct x. do 2 depelim ctapes.
+      exists x0, (mk_mconfig cstate0 h0). cbn in *. 
+      unfold loopM, TM.loopM in *.
+      eapply loop_lift with (lift := @f_config _ _) in H.
+      cbn in H. rewrite <- H.
+      f_equal.
+      * reflexivity.
+      * intros. cbn. depelim x. depelim ctapes. depelim ctapes. reflexivity.
+      * intros. cbn. depelim x. depelim ctapes. depelim ctapes. cbn in *.
+        unfold step, TM.step. cbn.
+        destruct (trans0 (cstate1, [|current h1|])) eqn:E.
+        depelim t. depelim t. cbn. rewrite E. reflexivity.
+    + intros (? & ? & ?).
+      cbn in *. destruct x0.
+      exists (TM.mk_mconfig cstate0 [| ctape0 |]), x.
+      unfold TM.loopM, loopM in *.
+      eapply (loop_lift (lift := fun '(mk_mconfig a b) => @TM.mk_mconfig sig states0 1 a [| b |])) in H.
+      rewrite <- H.
+      f_equal.
+      * now intros [].
+      * intros [] ?. unfold step, TM.step, current_chars.
+        cbn. destruct (trans0 (cstate1, [|current ctape1|])) eqn:E.
+        depelim t. depelim t. reflexivity.
+Qed.
+
+Inductive test (m n : nat) : Type :=
+  B : test m (n + 1) -> test m n.
+
