Makefile
@@ -1,0 +1,15 @@
+all:
+	+make -C external all
+	+make -C theories all
+
+clean:
+	+make -C theories clean
+
+realclean:
+	+make -C external clean
+	+make -C theories clean
+
+html:
+	+make -C theories website
+
+.PHONY: all html clean realclean
